Exercises 1 and 2

teaching/taltech2018/ex/ex2/Stack.fst
@@ -7,22 +7,23 @@ module Stack
    In this exercise you will practice writing purely functional programs against interfaces.
 
    The goal is for you to define a small library of integer-valued stacks (if you haven't 
-   seen stacks before, see e.g. https://en.wikipedia.org/wiki/Stack_(abstract_data_type)). 
+   seen stacks before, see e.g. https://en.wikipedia.org/wiki/Stack_(abstract_data_type)), 
+   and use it in the client code in `StackClient.fst`, including verifying simple properties.
 
-   Task 1: Below define all the types, functions, and lemmas required by the interface 
-           of stacks (`Stack.fsti`) so that this file (`Stack.fst`) verifies/typechecks.
+   Task 1: In the space below, define all the types, functions, and lemmas required by the  
+           interface `Stack.fsti` so that this file (`Stack.fst`) verifies (i.e., typechecks).
 
            Note: When using the interactive fstar-mode, F* will not complain if you haven't
            defined all the functions and lemmas required by `Stack.fsti` (but it will 
            complain if you define them in different order than stated in `Stack.fsti`). 
            The former is so because of the interactive nature of using fstar-mode, and the 
-           possibility of extending the interface and the implementation in parallel.
+           possibility of extending the interface and the implementation code in parallel.
            Thus, to ensure that your implementation of stacks truly reflects the interface, 
            you should run F* from the command line with `fstar.exe` on the current file.
 
    Task 2: Remove the [@expect_failure] attribute in `StackClient.fst` and try to verify 
-           that file. The verification will fail because `StackClient.fst` cannot see 
-           the parts of `Stack.fst` not exposed by its interface `Stack.fsti`. 
+           said file. The verification will fail because `StackClient.fst` cannot see the 
+           implementation details of `Stack.fst` not exposed by its interface `Stack.fsti`. 
 
    Task 3: To overcome the failure in Task 2, extend the interface `Stack.fsti` with 
            additional properties (lemmas) about the behaviour of stacks, and of course 
@@ -33,35 +34,3 @@ module Stack
            explicitly in `main ()`, you need to annotate them with SMT-patterns ([SMTPat (...)]).
 
 *)
-
-let stack = list int
-  
-let empty = []
-
-let is_empty xs = match xs with
-                  | [] -> true
-                  | x::xs' -> false
-
-let push x xs = x :: xs
-
-let pop xs = match xs with
-             | [] -> None
-             | x::xs' -> Some xs'
-
-let top xs = match xs with
-             | [] -> None
-             | x::xs' -> Some x
-
-let lemma_empty_is_empty () = ()
-
-let lemma_push_is_not_empty s i = ()
-
-let lemma_is_not_empty_top_some s = ()
-
-let lemma_is_not_empty_pop_some s = ()
-
-let lemma_push_top s i = ()
-
-let lemma_push_pop s i = ()
-
-let lemma_top_pop_push s = ()
