teaching/taltech2018/ex/ex2/Stack.fsti
@@ -1,0 +1,23 @@
+module Stack
+
+(*
+
+   Exercise 2.
+
+   See `Stack.fst` for details.
+
+*)
+
+val stack : Type0
+
+val empty : stack
+
+val is_empty : stack -> GTot bool
+
+val push : int -> stack -> stack
+
+val pop : stack -> option stack
+
+val top : stack -> option int
+
+val lemma_empty_is_empty : unit -> Lemma (is_empty (empty))
