teaching/taltech2018/ex/ex2/StackClient.fst
@@ -10,6 +10,7 @@ open Stack
 
 *)
 
+[@expect_failure]
 let main() =
 
   let s0 = empty (* <: stack *) in
